@prefix swe:   <urn:x-gsml-rdf:types> .
@prefix gsmlpp: <http://geosciml.org/ont/gsmlpp#> .
@prefix iso19150-2: <http://def.isotc211.org/iso19150/-2/2012/base#> .
@prefix owl:   <http://www.w3.org/2002/07/owl#> .
@prefix gsmlst: <http://geosciml.org/ont/gsmlst#> .
@prefix xsd:   <http://www.w3.org/2001/XMLSchema#> .
@prefix skos:  <http://www.w3.org/2004/02/skos/core#> .
@prefix rdfs:  <http://www.w3.org/2000/01/rdf-schema#> .
@prefix gsmlu: <http://geosciml.org/ont/gsmlu#> .
@prefix gsmlga: <http://geosciml.org/ont/gsmlga#> .
@prefix gsmlgt: <http://geosciml.org/ont/gsmlgt#> .
@prefix rdf:   <http://www.w3.org/1999/02/22-rdf-syntax-ns#> .
@prefix gsmlem: <http://geosciml.org/ont/gsmlem#> .
@prefix gsml:  <http://geosciml.org/ont/gsml#> .

gsmlst:totalDisplacement
        a                owl:ObjectProperty ;
        rdfs:range       gsmlst:DisplacementValue ;
        skos:definition  "Describes the total displacement DisplacementValues"@en .

gsmlst:geneticModel  a   owl:ObjectProperty ;
        rdfs:range       swe:Category ;
        skos:definition  "Specification of genetic model for fold, e.g. flexural slip, parallel"@en .

gsmlst:lineationType  a  owl:ObjectProperty ;
        rdfs:range       skos:Concept ;
        skos:definition  "Type of lineation.\r\nExamples include: flow lines, scratches, striae, slickenlines, linear arrangements of elongate components in sediments, elongate minerals, crinkles, and lines of intersection between penetrative planar structures."@en .

gsmlst:layerComposition
        a                owl:ObjectProperty ;
        rdfs:range       gsmlem:RockMaterial ;
        skos:definition  "Describes the rock material that may define compositional layering"@en .

gsmlst:Fracture  a             owl:Class ;
        rdfs:subClassOf        gsmlst:GeologicStructure ;
        iso19150-2:isAbstract  true ;
        skos:definition        "Fractures are cracks in the earth surface. If there is no displacement it is a joint. If there is displacement and you are in the brittle zone it is a fault. In the ductile zone, a fracture with displacement with fracture is called a shear. FaultSurface as a separate class is not considered necessary for GeoSciML 2.\r\nRecording observations on FaultSurface should be in observation and measurement. The observation needs to be able to distinguish the type of measurement made (PropertyType)"@en .

gsmlst:Foliation.mineralElement
        a                owl:ObjectProperty ;
        rdfs:domain      gsmlst:Foliation ;
        rdfs:range       gsmlem:Mineral ;
        skos:definition  "The mineral that defines the foliation"@en .

gsmlst:contactCharacter
        a                owl:ObjectProperty ;
        rdfs:range       swe:Category ;
        skos:definition  "The character of the boundary, as opposed to its type. e.g. abrupt, gradational"@en .

gsmlst:amplitude  a      owl:ObjectProperty ;
        rdfs:range       swe:QuantityRange ;
        skos:definition  "length from line segment connecting inflection points on adjacent fold limbs to the intervening fold hinge"@en .

gsmlst:correlatesWith
        a           owl:ObjectProperty ;
        rdfs:range  gsmlgt:GeochronologicBoundary .

gsmlst:Contact.orientation
        a                owl:ObjectProperty ;
        rdfs:domain      gsmlst:Contact ;
        rdfs:range       gsmlu:CGI_PlanarOrientation ;
        skos:definition  "orientation of the contact surface"@en .

gsmlst:DisplacementEvent
        a                owl:Class ;
        rdfs:subClassOf  gsmlga:GeologicEvent ;
        rdfs:subClassOf  [ a                  owl:Restriction ;
                           owl:allValuesFrom  gsmlst:DisplacementValue ;
                           owl:onProperty     gsmlst:incrementalDisplacement
                         ] ;
        skos:definition  "A description of the age, environment and process of a shear displacement event"@en .

gsmlst:Layering  a       owl:Class ;
        rdfs:subClassOf  gsmlst:Foliation ;
        rdfs:subClassOf  [ a                  owl:Restriction ;
                           owl:allValuesFrom  gsmlem:RockMaterial ;
                           owl:onProperty     gsmlst:layerComposition
                         ] ;
        skos:definition  "Planar foliation defined by a tabular succession of layers > 5 mm thick. This definition is based on the proposed definition of gneiss by the NADM Science Language Technical Team, so that the GeologicStructure characteristic of gneiss is layering. The committee discussed the possibility that layering should be considered a kind of foliation, but the majority opinion was that it is a different kind of structure.  Kept so that instance documents have a \"Layering\" tag"@en .

gsmlst:interLimbAngle
        a                owl:ObjectProperty ;
        rdfs:range       swe:Category ;
        skos:definition  "Specify using a tightness term (gentle (120-180), open (70-120), close (30-70), tight (10-30), isoclinal (0-10))"@en .

gsmlst:Lineation.definingElement
        a                owl:ObjectProperty ;
        rdfs:domain      gsmlst:Lineation ;
        rdfs:range       swe:Category ;
        skos:definition  "Kinds of describable inhomogeneity in a rock body that may define a GeologicStructure.   Examples include Oriented Particle."@en .

gsmlst:hingeLineCurvature
        a                owl:ObjectProperty ;
        rdfs:range       swe:Category ;
        skos:definition  "variation in orientation of fold hinge along trend of fold, distinguish sheath from cylindrical folds. Specify with terminology eg sheath, dome, basin, cylindrical."@en .

gsmlst:throw  a          owl:ObjectProperty ;
        rdfs:range       gsmlu:CGI_Vector ;
        skos:definition  "vertical component of slip"@en .

gsmlst:Lineation  a      owl:Class ;
        rdfs:subClassOf  gsmlst:GeologicStructure ;
        rdfs:subClassOf  [ a                  owl:Restriction ;
                           owl:allValuesFrom  gsmlu:CGI_LinearOrientation ;
                           owl:onProperty     gsmlst:Lineation.orientation
                         ] ;
        rdfs:subClassOf  [ a                  owl:Restriction ;
                           owl:allValuesFrom  gsmlem:Mineral ;
                           owl:onProperty     gsmlst:Lineation.mineralElement
                         ] ;
        rdfs:subClassOf  [ a                  owl:Restriction ;
                           owl:allValuesFrom  swe:Category ;
                           owl:onProperty     gsmlst:Lineation.intensity
                         ] ;
        rdfs:subClassOf  [ a                  owl:Restriction ;
                           owl:allValuesFrom  skos:Concept ;
                           owl:onProperty     gsmlst:lineationType
                         ] ;
        rdfs:subClassOf  [ a                  owl:Restriction ;
                           owl:allValuesFrom  swe:Category ;
                           owl:onProperty     gsmlst:Lineation.definingElement
                         ] ;
        skos:definition  "GeologicStructure defined by aligned elongate elements. Lineation connotes a pervasive linear structure. Includes: flow lines, scratches, striae, slickenlines, linear arrangements of\r\nelongate components in sediments, fold hinges (when abundant and closely spaced), elongate minerals, crinkles, and lines of intersection between penetrative planar structures.\r\n\r\nClass also includes discrete linear structures like boudin, channel axis, tool marks."@en .

gsmlst:structureType  a  owl:ObjectProperty ;
        rdfs:range       skos:Concept ;
        skos:definition  "The type of non oriented structure.  Examples include miarolitic cavity, flame structure, load cast, shatter cone, trace fossil, fossil mold"@en .

gsmlst:hingeLineOrientation
        a                owl:ObjectProperty ;
        rdfs:range       gsmlu:CGI_LinearOrientation ;
        skos:definition  "Specification of hinge line orientation for fold. CGI_LinearOrientation allows for a term value specification or a numeric specification of either or both the trend and plunge of hinge line. kHinge plunge term examples: sub-vertical, steeply plunging, ... sub-horizontal, reclined and vertical for special cases in which hinge plunge is close to axial surface dip. 0..* cardinality allows for both a numeric specification a term specification."@en .

gsmlst:DisplacementValue
        a                owl:Class ;
        rdfs:subClassOf  [ a                  owl:Restriction ;
                           owl:allValuesFrom  gsmlst:DisplacementEvent ;
                           owl:onProperty     gsmlst:displacementEvent
                         ] ;
        rdfs:subClassOf  [ a                  owl:Restriction ;
                           owl:allValuesFrom  skos:Concept ;
                           owl:onProperty     gsmlst:movementType
                         ] ;
        rdfs:subClassOf  [ a                  owl:Restriction ;
                           owl:allValuesFrom  skos:Concept ;
                           owl:onProperty     gsmlst:movementSense
                         ] ;
        rdfs:subClassOf  [ a                  owl:Restriction ;
                           owl:allValuesFrom  gsmlu:CGI_LinearOrientation ;
                           owl:onProperty     gsmlst:hangingWallDirection
                         ] ;
        skos:definition  "Trying to express the displacement on a fault with respect to a planar approximation of its shape"@en .

gsmlst:spacing  a        owl:ObjectProperty ;
        rdfs:range       swe:QuantityRange ;
        skos:definition  "linear dimension representing the thickness of foliation domains. Also use for thickness of layers of a given composition"@en .

gsmlst:slipComponent  a  owl:ObjectProperty ;
        rdfs:range       gsmlst:SlipComponents ;
        skos:definition  "Specifies the value of the individual slip components."@en .

gsmlst:Foliation.intensity
        a                owl:ObjectProperty ;
        rdfs:domain      gsmlst:Foliation ;
        rdfs:range       swe:Category ;
        skos:definition  "How well the foliation is developed. Terms such as weak, moderate, strong."@en .

gsmlst:foldSystemMember
        a                owl:ObjectProperty ;
        rdfs:range       gsmlst:Fold ;
        skos:definition  "Specifies the Fold that is a member of the FoldSystem"@en .

gsmlst:continuity  a     owl:ObjectProperty ;
        rdfs:range       swe:Category ;
        skos:definition  "terms to distinguish continuous vs. disjunct cleavages"@en .

gsmlst:hangingWallDirection
        a                owl:ObjectProperty ;
        rdfs:range       gsmlu:CGI_LinearOrientation ;
        skos:definition  "Normally the compass quadrant indicating the hangingwall side of the fault-system for faults that are steep enough to define a hanging-wall on the map trace"@en .

gsmlst:Contact  a        owl:Class ;
        rdfs:subClassOf  gsmlst:GeologicStructure ;
        rdfs:subClassOf  [ a                  owl:Restriction ;
                           owl:allValuesFrom  gsmlgt:GeochronologicBoundary ;
                           owl:onProperty     gsmlst:correlatesWith
                         ] ;
        rdfs:subClassOf  [ a                  owl:Restriction ;
                           owl:allValuesFrom  gsmlu:CGI_PlanarOrientation ;
                           owl:onProperty     gsmlst:Contact.orientation
                         ] ;
        rdfs:subClassOf  [ a                  owl:Restriction ;
                           owl:allValuesFrom  skos:Concept ;
                           owl:onProperty     gsmlst:contactType
                         ] ;
        rdfs:subClassOf  [ a                  owl:Restriction ;
                           owl:allValuesFrom  swe:Category ;
                           owl:onProperty     gsmlst:contactCharacter
                         ] ;
        skos:definition  "Very general concept representing any kind of surface separating two geologic units including primary boundaries such as depositional contacts, all kinds of unconformities, intrusive contacts, and gradational contacts, as well as faults that separate geologic units.\r\n\r\nPermeability of contacts still needs to be modeled; considered out of scope for GeoSciML2.\r\n\r\nBedding measured as discrete surfaces in the case that those are the feature of interest (e.g. individual cross set surfaces for paleocurrent analysis) should be represented here."@en .

gsmlst:separation  a     owl:ObjectProperty ;
        rdfs:range       gsmlu:CGI_Vector ;
        skos:definition  "Reported apparent offset of planar feature, report as vector."@en .

gsmlst:deformationStyle
        a                owl:ObjectProperty ;
        rdfs:range       skos:Concept ;
        skos:definition  "A mandatory element referring to a vocabulary of terms to describe the style of deformation, ie brittle (fault, breccia), ductile (shear), brittle-ductile, unknown."@en .

gsmlst:Foliation  a      owl:Class ;
        rdfs:subClassOf  gsmlst:GeologicStructure ;
        rdfs:subClassOf  [ a                  owl:Restriction ;
                           owl:allValuesFrom  swe:Category ;
                           owl:onProperty     gsmlst:Foliation.intensity
                         ] ;
        rdfs:subClassOf  [ a                  owl:Restriction ;
                           owl:allValuesFrom  gsmlem:Mineral ;
                           owl:onProperty     gsmlst:Foliation.mineralElement
                         ] ;
        rdfs:subClassOf  [ a                  owl:Restriction ;
                           owl:allValuesFrom  swe:QuantityRange ;
                           owl:onProperty     gsmlst:spacing
                         ] ;
        rdfs:subClassOf  [ a                  owl:Restriction ;
                           owl:allValuesFrom  swe:Category ;
                           owl:onProperty     gsmlst:continuity
                         ] ;
        rdfs:subClassOf  [ a                  owl:Restriction ;
                           owl:allValuesFrom  skos:Concept ;
                           owl:onProperty     gsmlst:foliationType
                         ] ;
        rdfs:subClassOf  [ a                  owl:Restriction ;
                           owl:allValuesFrom  gsmlu:CGI_PlanarOrientation ;
                           owl:onProperty     gsmlst:Foliation.orientation
                         ] ;
        rdfs:subClassOf  [ a                  owl:Restriction ;
                           owl:allValuesFrom  swe:Category ;
                           owl:onProperty     gsmlst:Foliation.definingElement
                         ] ;
        skos:definition  "A planar arrangement of textural or structural features in any type of rock. Includes any of a wide variety of penetrative planar geological structures that may be present in a rock.  Examples include schistosity, mylonitic foliation, penetrative bedding structure (lamination), and cleavage.  Following the proposed definition of gneiss by the NADM Science Language Technical Team, penetrative planar foliation defined by layers > 5 mm thick is considered Layering. \r\nBedding as a fabric representing the average orientation of paleodepositional surface should be encoded through the foliationType; might apply to bedding that is layering or a foliation without layering (e.g. clast alignment in amalgamated beds)."@en .

gsmlst:limbShape  a      owl:ObjectProperty ;
        rdfs:range       swe:Category ;
        skos:definition  "straight vs curved limbs, eg kink, chevron, sinusoidal, box"@en .

gsmlst:contactType  a    owl:ObjectProperty ;
        rdfs:range       skos:Concept ;
        skos:definition  "Classifies the contact (eg intrusive, unconformity, bedding surface, lithologic boundary, phase boundary)"@en .

gsmlst:movementType  a   owl:ObjectProperty ;
        rdfs:range       skos:Concept ;
        skos:definition  "Defines the type of movement  (eg dip-slip, strike-slip)"@en .

gsmlst:SeparationValue
        a                owl:Class ;
        rdfs:subClassOf  gsmlst:DisplacementValue ;
        rdfs:subClassOf  [ a                  owl:Restriction ;
                           owl:allValuesFrom  gsmlu:CGI_Vector ;
                           owl:onProperty     gsmlst:separation
                         ] ;
        skos:definition  "The amount of separation displacement"@en .

gsmlst:foliationType  a  owl:ObjectProperty ;
        rdfs:range       skos:Concept ;
        skos:definition  "Specifies the type of foliation.  Examples include crenulation cleavage, slaty cleavage, schistosity"@en .

gsmlst:Fold.system  a    owl:ObjectProperty ;
        rdfs:domain      gsmlst:Fold ;
        rdfs:range       gsmlst:FoldSystem ;
        skos:definition  "Describes a broader system of folds to which an individual fold may belong"@en .

gsmlst:symmetry  a       owl:ObjectProperty ;
        rdfs:range       swe:Category ;
        skos:definition  "Concordance or discordance of bisecting surface and axial surface, or ratio of length of limbs. Folded surface may have asymmetry defined by limb length ratio if inflection points are defined. Defintion based on bisecting surface/axial surface angle depends on having multiple surfaces defined such that the axial surface may be identified. (symmetric, assymetric)"@en .

gsmlst:ShearDisplacementStructure.system
        a                owl:ObjectProperty ;
        rdfs:domain      gsmlst:ShearDisplacementStructure ;
        rdfs:range       gsmlst:FaultSystem ;
        skos:definition  "Describes the fault system to which a ShearDisplacementStructures belongs"@en .

gsmlst:DefiningStructure
        a                owl:Class ;
        rdfs:subClassOf  gsml:GeologicFeatureRelation ;
        skos:definition  "Describes the related GeologicStructure which defines a DeformationUnit. That is, a geologic unit defined by its deformation character, eg a shear zone."@en .

gsmlst:FaultSystem  a    owl:Class ;
        rdfs:subClassOf  gsmlst:ShearDisplacementStructure ;
        rdfs:subClassOf  [ a                  owl:Restriction ;
                           owl:allValuesFrom  gsmlst:ShearDisplacementStructure ;
                           owl:onProperty     gsmlst:faultSystemMember
                         ] ;
        skos:definition  "A composite structure that is an aggregation of genetically related instances of Faults and/or DuctileShearStructures. A FaultSystem is composed of individually identified and mapped Faults and/or DuctileShearStructures that are considered distinct ShearDisplacementStructures, that generally form overlapping, anastomosing patterns in which, at any point along the fault system, multiple fault strands are identified and each considered important at the scale of description. Displacement and other descriptive data may be assigned at the 'fault segment', 'fault', or 'fault system level'."@en .

gsmlst:horizontalSlip
        a                owl:ObjectProperty ;
        rdfs:range       gsmlu:CGI_Vector ;
        skos:definition  "slip component that is horizontal and parallel to strike of the fault"@en .

gsmlst:NonDirectionalStructure
        a                owl:Class ;
        rdfs:subClassOf  gsmlst:GeologicStructure ;
        rdfs:subClassOf  [ a                  owl:Restriction ;
                           owl:allValuesFrom  skos:Concept ;
                           owl:onProperty     gsmlst:structureType
                         ] ;
        skos:definition  "Structures present in geology that do not have a preferred orientation\r\nIncludes small-scale structures that are characteristic of the geologic unit, e.g. herringbone crossbedding, mudcracks, graded bedding, planar lamination, miarolitic cavities, nebulitic structure, trace fossils, fossil molds"@en .

gsmlst:movementSense  a  owl:ObjectProperty ;
        rdfs:range       skos:Concept ;
        skos:definition  "eg, dextral, sinistral"@en .

gsmlst:wavelength  a     owl:ObjectProperty ;
        rdfs:range       swe:QuantityRange ;
        skos:definition  "Quantitative specification of length between adjacent antiforms (or synforms) in a fold train."@en .

gsmlst:Lineation.intensity
        a                owl:ObjectProperty ;
        rdfs:domain      gsmlst:Lineation ;
        rdfs:range       swe:Category ;
        skos:definition  "How well the lineation is developed. Terms such as weak, moderate, strong."@en .

gsmlst:periodic  a       owl:DatatypeProperty ;
        rdfs:range       xsd:boolean ;
        skos:definition  "True if fold hinges in train are regularly spaced."@en .

<http://geosciml.org/ont/gsmlst>
        a                owl:Ontology ;
        owl:imports      <http://geosciml.org/ont/gsmlu> , <http://geosciml.org/ont/gsmlga> , <http://geosciml.org/ont/gsml> , <http://schemas.geosciml.org/rdf/types.ttl> , <http://geosciml.org/ont/gsmlgt> , <http://geosciml.org/ont/gsmlem> , <http://geosciml.org/ont/gsmlpp> ;
        owl:versionIRI   "http://geosciml.org/ont/gsmlst/3.2.0" ;
        owl:versionInfo  "3.2.0" ;
        skos:definition  "GeologicStructures are a configuration of matter in the Earth based on describable inhomogeneity, pattern, or fracture in an Earth Material.  The scale of geological structures ranges from microscopic (micron-scale) to megascopic (km-scale). Examples of such inhomogeneities include fractures, mineral grain boundaries, and boundaries between parts of the rock with different particle geometry (texture) or composition. Geologic structure is grounded in relationships between parts of a rock or rock body. As used here, it includes sedimentary structures. The identity of a Geologic Structure is independent of the material that is the substrate for the structure. There are almost always strong dependencies between the nature of the Earth Material substrate and the kinds of Geological Structure that may be present. A disaggregated heap of particles does not have structure, and can only be described in terms of the mineralogy and geometrical character of the constituent particles.  Geologic Structures are more likely to be found in, and are more persistent in, consolidated materials than in unconsolidated materials. Properties like \"clast-supported\", \"matrix-supported\", and \"graded bed\" that do not involve orientation are considered kinds of Geologic Structure because they depend on the configuration of parts of a rock body."@en .

gsmlst:FoldSystem  a     owl:Class ;
        rdfs:subClassOf  gsmlst:GeologicStructure ;
        rdfs:subClassOf  [ a                  owl:Restriction ;
                           owl:allValuesFrom  gsmlst:Fold ;
                           owl:onProperty     gsmlst:foldSystemMember
                         ] ;
        rdfs:subClassOf  [ a                  owl:Restriction ;
                           owl:allValuesFrom  swe:QuantityRange ;
                           owl:onProperty     gsmlst:wavelength
                         ] ;
        rdfs:subClassOf  [ a                  owl:Restriction ;
                           owl:allValuesFrom  xsd:boolean ;
                           owl:onProperty     gsmlst:periodic
                         ] ;
        skos:definition  "A collection of congruent folds  (axis and axial surface are parallel) produced by the same tectonic event. Sometimes referred to as a \"Fold Train\"."@en .

gsmlst:Foliation.definingElement
        a                owl:ObjectProperty ;
        rdfs:domain      gsmlst:Foliation ;
        rdfs:range       swe:Category ;
        skos:definition  "Kinds of describable inhomogeneity in a rock body that may define a GeologicStructure.   Examples include Discontinuity, Shaped Surface, Oriented Particle, Material Boundary, and Layer."@en .

gsmlst:Joint  a          owl:Class ;
        rdfs:subClassOf  gsmlst:Fracture ;
        skos:definition  "Fracture across which there is no displacement at the scale of interest."@en .

gsmlst:incrementalDisplacement
        a           owl:ObjectProperty ;
        rdfs:range  gsmlst:DisplacementValue .

gsmlst:hingeShape  a     owl:ObjectProperty ;
        rdfs:range       swe:Category ;
        skos:definition  "Rounded vs. angular hinge zones; has to do with the proportion of the wavelength that is considered part of hinge"@en .

gsmlst:faultType  a      owl:ObjectProperty ;
        rdfs:range       skos:Concept ;
        skos:definition  "Refers to a vocabulary of terms describing the type of shear displacement structure (eg; thrust fault, normal fault, wrench fault)."@en .

gsmlst:Lineation.mineralElement
        a                owl:ObjectProperty ;
        rdfs:domain      gsmlst:Lineation ;
        rdfs:range       gsmlem:Mineral ;
        skos:definition  "Mineral that defines the lineation"@en .

gsmlst:ShearDisplacementStructure
        a                owl:Class ;
        rdfs:subClassOf  gsmlst:GeologicStructure ;
        rdfs:subClassOf  [ a                  owl:Restriction ;
                           owl:allValuesFrom  gsmlst:FaultSystem ;
                           owl:onProperty     gsmlst:ShearDisplacementStructure.system
                         ] ;
        rdfs:subClassOf  [ a                  owl:Restriction ;
                           owl:allValuesFrom  gsmlpp:PhysicalDescription ;
                           owl:onProperty     gsmlst:physicalProperty
                         ] ;
        rdfs:subClassOf  [ a                  owl:Restriction ;
                           owl:allValuesFrom  gsmlst:DisplacementValue ;
                           owl:onProperty     gsmlst:totalDisplacement
                         ] ;
        rdfs:subClassOf  [ a                  owl:Restriction ;
                           owl:allValuesFrom  gsmlu:CGI_PlanarOrientation ;
                           owl:onProperty     gsmlst:planeOrientation
                         ] ;
        rdfs:subClassOf  [ a                  owl:Restriction ;
                           owl:allValuesFrom  skos:Concept ;
                           owl:onProperty     gsmlst:deformationStyle
                         ] ;
        rdfs:subClassOf  [ a                  owl:Restriction ;
                           owl:allValuesFrom  skos:Concept ;
                           owl:onProperty     gsmlst:faultType
                         ] ;
        skos:definition  "A shear displacement structure includes all brittle to ductile style structures along which displacement has occurred, from a simple, single 'planar' brittle or ductile surface to a fault system comprised of 10's of strands of both brittle and ductile nature. This structure may have some significant thickness (a deformation zone) and have an associated body of deformed rock that may be considered a DeformationUnit"@en .

gsmlst:GeologicStructure
        a                      owl:Class ;
        rdfs:subClassOf        gsml:GeologicFeature ;
        iso19150-2:isAbstract  true ;
        skos:definition        "A configuration of matter in the Earth based on describable inhomogeneity, pattern, or fracture in an EarthMaterial. \r\nThe identity of a GeologicStructure is independent of the material that is the substrate for the structure. \r\nProperties like \"clast-supported\",  \"matrix-supported\", and \"graded bed\" that do not involve orientation are considered kinds of GeologicStructure \r\nbecause they depend on the configuration of parts of a rock body. Includes sedimentary structures.\r\nThe general GeologicRelation is used to associate penetrative GeologicStructures with GeologicUnits."@en .

gsmlst:physicalProperty
        a           owl:ObjectProperty ;
        rdfs:range  gsmlpp:PhysicalDescription .

gsmlst:displacementEvent
        a                owl:ObjectProperty ;
        rdfs:range       gsmlst:DisplacementEvent ;
        skos:definition  "A description of the age, environment and process of a shear displacement event"@en .

gsmlst:axialSurfaceOrientation
        a                owl:ObjectProperty ;
        rdfs:range       gsmlu:CGI_PlanarOrientation ;
        skos:definition  "This is used to characterize the geometry of a fold. The axial surface of a particular fold may be located based on observations of the folded geologic structure, but in general it has no direct physical manifestions. As a geologic surface, it has geometric properties, including orientation, which may be specified by observations at one or more locations, or generalized using terminology (upright, inclined, reclined, recumbent, overturned). Dip and Dip Direction are one approach to specifying the value."@en .

gsmlst:planeOrientation
        a                owl:ObjectProperty ;
        rdfs:range       gsmlu:CGI_PlanarOrientation ;
        skos:definition  "Allows capturing the orientation of the plane of the structure"@en .

gsmlst:netSlip  a        owl:ObjectProperty ;
        rdfs:range       gsmlu:CGI_Vector ;
        skos:definition  "The value of the net slip"@en .

gsmlst:profileType  a    owl:ObjectProperty ;
        rdfs:range       skos:Concept ;
        skos:definition  "Terminology specifying concave/convex geometry of fold relative to earth surface, and relationship to younging direction in folded strata if known. (eg; antiform, synform, neutral, anticline, syncline, monocline, ptygmatic)"@en .

gsmlst:faultSystemMember
        a                owl:ObjectProperty ;
        rdfs:range       gsmlst:ShearDisplacementStructure ;
        skos:definition  "Specifies the ShearDisplacementStructures that are members of the FaultSystem"@en .

gsmlst:Lineation.orientation
        a                owl:ObjectProperty ;
        rdfs:domain      gsmlst:Lineation ;
        rdfs:range       gsmlu:CGI_LinearOrientation ;
        skos:definition  "Orientation of the lineation"@en .

gsmlst:span  a           owl:ObjectProperty ;
        rdfs:range       swe:QuantityRange ;
        skos:definition  "linear distance between inflection points in a single fold"@en .

gsmlst:heave  a          owl:ObjectProperty ;
        rdfs:range       gsmlu:CGI_Vector ;
        skos:definition  "component of slip in the horizontal, and perpendicular to the strike of the fault"@en .

gsmlst:BoundaryRelationship
        a                owl:Class ;
        rdfs:subClassOf  gsml:GeologicFeatureRelation ;
        skos:definition  "Defines the two GeologicUnits that make up the relationship described by the Contact"@en .

gsmlst:Fold  a           owl:Class ;
        rdfs:subClassOf  gsmlst:GeologicStructure ;
        rdfs:subClassOf  [ a                  owl:Restriction ;
                           owl:allValuesFrom  gsmlu:CGI_LinearOrientation ;
                           owl:onProperty     gsmlst:hingeLineOrientation
                         ] ;
        rdfs:subClassOf  [ a                  owl:Restriction ;
                           owl:allValuesFrom  swe:QuantityRange ;
                           owl:onProperty     gsmlst:amplitude
                         ] ;
        rdfs:subClassOf  [ a                  owl:Restriction ;
                           owl:allValuesFrom  swe:Category ;
                           owl:onProperty     gsmlst:symmetry
                         ] ;
        rdfs:subClassOf  [ a                  owl:Restriction ;
                           owl:allValuesFrom  swe:Category ;
                           owl:onProperty     gsmlst:limbShape
                         ] ;
        rdfs:subClassOf  [ a                  owl:Restriction ;
                           owl:allValuesFrom  gsmlu:CGI_PlanarOrientation ;
                           owl:onProperty     gsmlst:axialSurfaceOrientation
                         ] ;
        rdfs:subClassOf  [ a                  owl:Restriction ;
                           owl:allValuesFrom  gsmlst:FoldSystem ;
                           owl:onProperty     gsmlst:Fold.system
                         ] ;
        rdfs:subClassOf  [ a                  owl:Restriction ;
                           owl:allValuesFrom  skos:Concept ;
                           owl:onProperty     gsmlst:profileType
                         ] ;
        rdfs:subClassOf  [ a                  owl:Restriction ;
                           owl:allValuesFrom  swe:QuantityRange ;
                           owl:onProperty     gsmlst:span
                         ] ;
        rdfs:subClassOf  [ a                  owl:Restriction ;
                           owl:allValuesFrom  swe:Category ;
                           owl:onProperty     gsmlst:geneticModel
                         ] ;
        rdfs:subClassOf  [ a                  owl:Restriction ;
                           owl:allValuesFrom  swe:Category ;
                           owl:onProperty     gsmlst:hingeLineCurvature
                         ] ;
        rdfs:subClassOf  [ a                  owl:Restriction ;
                           owl:allValuesFrom  swe:Category ;
                           owl:onProperty     gsmlst:hingeShape
                         ] ;
        rdfs:subClassOf  [ a                  owl:Restriction ;
                           owl:allValuesFrom  swe:Category ;
                           owl:onProperty     gsmlst:interLimbAngle
                         ] ;
        skos:definition  "One or more systematically curved layers, surfaces, or lines in a rock body. Fold denotes a structure formed by the deformation of a GeologicStructure to form a structure that may be described by the translation of an abstract line (the fold axis) parallel to itself along some curvilinear path (the fold profile). Folds have a hinge zone (zone of maximum curvature along the surface) and limbs (parts of the deformed surface not in the hinge zone).  Folds are described by an axial surface, hinge line , profile geometry, the solid angle between the limbs, and the relationships between adjacent folded surfaces if the folded structure is a Layering fabric (similar, parallel)."@en .

gsmlst:NetSlipValue  a   owl:Class ;
        rdfs:subClassOf  gsmlst:DisplacementValue ;
        rdfs:subClassOf  [ a                  owl:Restriction ;
                           owl:allValuesFrom  gsmlst:SlipComponents ;
                           owl:onProperty     gsmlst:slipComponent
                         ] ;
        rdfs:subClassOf  [ a                  owl:Restriction ;
                           owl:allValuesFrom  gsmlu:CGI_Vector ;
                           owl:onProperty     gsmlst:netSlip
                         ] ;
        skos:definition  "The total amount of slip displacement"@en .

gsmlst:SlipComponents
        a                owl:Class ;
        rdfs:subClassOf  gsmlst:DisplacementValue ;
        rdfs:subClassOf  [ a                  owl:Restriction ;
                           owl:allValuesFrom  gsmlu:CGI_Vector ;
                           owl:onProperty     gsmlst:throw
                         ] ;
        rdfs:subClassOf  [ a                  owl:Restriction ;
                           owl:allValuesFrom  gsmlu:CGI_Vector ;
                           owl:onProperty     gsmlst:horizontalSlip
                         ] ;
        rdfs:subClassOf  [ a                  owl:Restriction ;
                           owl:allValuesFrom  gsmlu:CGI_Vector ;
                           owl:onProperty     gsmlst:heave
                         ] ;
        skos:definition  "Representation of slip as vector resolved into components resolved into reference frame in which horizontal axes are parallel and perpendicular to the strike of the fault.  At least one of heave, horizontalSlip, or throw must not be null."@en .

gsmlst:Foliation.orientation
        a                owl:ObjectProperty ;
        rdfs:domain      gsmlst:Foliation ;
        rdfs:range       gsmlu:CGI_PlanarOrientation ;
        skos:definition  "The planar orientation of the foliation"@en .
