@prefix swe:   <urn:x-gsml-rdf:types> .
@prefix sf:    <http://def.seegrid.csiro.au/isotc211/iso19156/2011/sampling> .
@prefix gsp:   <http://www.opengis.net/ont/geosparql#> .
@prefix rdf:   <http://www.w3.org/1999/02/22-rdf-syntax-ns#> .
@prefix owl:   <http://www.w3.org/2002/07/owl#> .
@prefix xsd:   <http://www.w3.org/2001/XMLSchema#> .
@prefix skos:  <http://www.w3.org/2004/02/skos/core#> .
@prefix rdfs:  <http://www.w3.org/2000/01/rdf-schema#> .
@prefix gsml:  <http://geosciml.org/ont/gsml#> .
@prefix time:  <http://www.w3.org/2006/time#> .
@prefix gsmlbh: <http://geosciml.org/ont/gsmlbh#> .

gsmlbh:BoreholeDetails
        a                owl:Class ;
        rdfs:subClassOf  [ a                  owl:Restriction ;
                           owl:allValuesFrom  skos:Concept ;
                           owl:onProperty     gsmlbh:purpose
                         ] ;
        rdfs:subClassOf  [ a                  owl:Restriction ;
                           owl:allValuesFrom  skos:Concept ;
                           owl:onProperty     gsmlbh:startPoint
                         ] ;
        rdfs:subClassOf  [ a                  owl:Restriction ;
                           owl:allValuesFrom  swe:Quantity ;
                           owl:onProperty     gsmlbh:boreholeLength
                         ] ;
        rdfs:subClassOf  [ a                  owl:Restriction ;
                           owl:allValuesFrom  time:Period ;
                           owl:onProperty     gsmlbh:dateOfDrilling
                         ] ;
        rdfs:subClassOf  [ a                  owl:Restriction ;
                           owl:allValuesFrom  skos:Concept ;
                           owl:onProperty     gsmlbh:driller
                         ] ;
        rdfs:subClassOf  [ a                  owl:Restriction ;
                           owl:allValuesFrom  skos:Concept ;
                           owl:onProperty     gsmlbh:boreholeMaterialCustodian
                         ] ;
        rdfs:subClassOf  [ a                  owl:Restriction ;
                           owl:allValuesFrom  skos:Concept ;
                           owl:onProperty     gsmlbh:operator
                         ] ;
        rdfs:subClassOf  [ a                  owl:Restriction ;
                           owl:allValuesFrom  skos:Concept ;
                           owl:onProperty     gsmlbh:dataCustodian
                         ] ;
        rdfs:subClassOf  [ a                  owl:Restriction ;
                           owl:allValuesFrom  skos:Concept ;
                           owl:onProperty     gsmlbh:inclinationType
                         ] ;
        skos:definition  "Borehole specific index (or metadata) information"@en .

gsmlbh:Borehole  a       owl:Class ;
        rdfs:subClassOf  sf:SF_SamplingCurve ;
        rdfs:subClassOf  [ a                  owl:Restriction ;
                           owl:allValuesFrom  gsmlbh:MappedInterval ;
                           owl:onProperty     gsmlbh:logElement
                         ] ;
        rdfs:subClassOf  [ a                  owl:Restriction ;
                           owl:allValuesFrom  gsmlbh:DrillingDetails ;
                           owl:onProperty     gsmlbh:downholeDrillingDetails
                         ] ;
        rdfs:subClassOf  [ a                  owl:Restriction ;
                           owl:allValuesFrom  gsmlbh:BoreholeDetails ;
                           owl:onProperty     gsmlbh:indexData
                         ] ;
        rdfs:subClassOf  [ a                  owl:Restriction ;
                           owl:allValuesFrom  gsmlbh:OriginPosition ;
                           owl:onProperty     gsmlbh:referenceLocation
                         ] ;
        skos:definition  "A borehole is the generalized term for any narrow shaft drilled in the ground, either vertically or horizontally."@en .

gsmlbh:drillingMethod
        a                owl:ObjectProperty ;
        rdfs:range       skos:Concept ;
        skos:definition  "Indicates the drilling method used. Appropriate terms would include rotary air blast; auger; diamond core; air core; etc"@en .

gsmlbh:dataCustodian  a  owl:ObjectProperty ;
        rdfs:range       skos:Concept ;
        skos:definition  "The custodian (person or organisation) that is the custodian of data pertaining to this borehole."@en .

gsmlbh:purpose  a        owl:ObjectProperty ;
        rdfs:range       skos:Concept ;
        skos:definition  "The purpose for which the borehole was drilled. eg, site investigation, mineral exploration, hydrocarbon exploration, water resources"@en .

gsmlbh:logElement  a     owl:ObjectProperty ;
        rdfs:range       gsmlbh:MappedInterval ;
        skos:definition  "Links to 1-D MappedFeature instances that are logged (interpreted) intervals within a borehole. This requirement is common in geoscience boreholes"@en .

gsmlbh:elevation  a      owl:ObjectProperty ;
        rdfs:range       gsp:Geometry ;
        skos:definition  "Compromise approach to supply elevation explictly for location; this is to allow for software that cannot process 3-D GM_Point. Use null if elevation is unknown. Direct position shall have a dimension of 1, and CRS will be a \"vertical\" CRS (e.g. EPSG CRSs in the range 5600-5799)."@en .

gsmlbh:intervalEnd  a    owl:ObjectProperty ;
        rdfs:range       swe:Quantity ;
        skos:definition  "The measured distance of the end of the mapped interval along the path of the borehole. The measured value must be greater than or equal to the intervalBegin value.  The \"intervalBegin\" and \"intervalEnd\" elements are added in version 3.2 as a measure to overcome problems with the delivery and queryability of 1D GML shapes via the \"interval\" element."@en .

gsmlbh:inclinationType
        a                owl:ObjectProperty ;
        rdfs:range       skos:Concept ;
        skos:definition  "Indicates the inclination of the borehole. Appropriate terms would include vertical; inclined up; inclined down, horizontal"@en .

gsmlbh:startPoint  a     owl:ObjectProperty ;
        rdfs:range       skos:Concept ;
        skos:definition  "Indicates the position relative to ground surface where the borehole commenced. Appropriate terms would include Drilled from Ground Surface; Drilled Underground;  Drilled from Quarry Floor etc"@en .

gsmlbh:boreholeLength
        a                owl:ObjectProperty ;
        rdfs:range       swe:Quantity ;
        skos:definition  "The \"length\" of a borehole will be determined by the data provider (ie, \"length\" can have different sources, like drillers measurement, loggers measurement, survey measurement, etc)"@en .

gsmlbh:dateOfDrilling
        a                owl:ObjectProperty ;
        rdfs:range       time:Period ;
        skos:definition  "The time period during which drilling of the borehole occurred."@en .

gsmlbh:driller  a        owl:ObjectProperty ;
        rdfs:range       skos:Concept ;
        skos:definition  "The organisation responsible for drilling the borehole (as opposed to commissioning the borehole)"@en .

gsmlbh:boreholeMaterialCustodian
        a                owl:ObjectProperty ;
        rdfs:range       skos:Concept ;
        skos:definition  "Organisation that is custodian of the core recovered from the borehole"@en .

gsmlbh:location  a       owl:ObjectProperty ;
        rdfs:range       gsp:Geometry ;
        skos:definition  "The location of the BoreholeCollar"@en .

gsmlbh:operator  a       owl:ObjectProperty ;
        rdfs:range       skos:Concept ;
        skos:definition  "Organisation responsible for commissioning the borehole (as opposed to drilling the borehole)"@en .

gsmlbh:boreholeDiameter
        a                owl:ObjectProperty ;
        rdfs:range       swe:Quantity ;
        skos:definition  "The diameter of the drilled hole"@en .

<http://geosciml.org/ont/gsmlbh>
        a                owl:Ontology ;
        owl:imports      <http://eelst.cs.unibo.it/apps/LODE/source?url=http://def.seegrid.csiro.au/isotc211/iso19156/2011/sampling.ttl> , <http://geosciml.org/ont/gsml> , <https://www.w3.org/2006/time> , <http://schemas.geosciml.org/rdf/types.ttl> , <http://www.opengis.net/ont/geosparql> ;
        owl:versionIRI   "http://geosciml.org/ont/gsmlbh/3.2.0" ;
        owl:versionInfo  "3.2.0" ;
        skos:definition  "The GeoSciML Borehole package contains model elements for representing Boreholes. This is primarily through re-use of standard components from the (external) Observations and Measurements package."@en .

gsmlbh:MappedInterval
        a                owl:Class ;
        rdfs:subClassOf  gsml:MappedFeature ;
        rdfs:subClassOf  [ a                  owl:Restriction ;
                           owl:allValuesFrom  swe:Quantity ;
                           owl:onProperty     gsmlbh:mappedIntervalEnd
                         ] ;
        rdfs:subClassOf  [ a                  owl:Restriction ;
                           owl:allValuesFrom  swe:Quantity ;
                           owl:onProperty     gsmlbh:mappedIntervalBegin
                         ] ;
        skos:definition  "A special kind of Mapped Feature whose shape is 1-D interval and uses the SRS of the containing borehole"@en .

gsmlbh:mappedIntervalEnd
        a                owl:ObjectProperty ;
        rdfs:range       swe:Quantity ;
        skos:definition  "The measured distance of the end of the mapped interval along the path of the borehole. The measured value must be greater than or equal to the mappedIntervalBegin value.  The \"mappedIntervalBegin\" and \"mappedIntervalEnd\" elements are added in version 3.2 as a measure to overcome problems with the delivery and queryability of 1D GML shapes via the \"shape\" property."@en .

gsmlbh:downholeDrillingDetails
        a                owl:ObjectProperty ;
        rdfs:range       gsmlbh:DrillingDetails ;
        skos:definition  "Specifies the drilling method and borehole diameter for intervals down the borehole"@en .

gsmlbh:intervalBegin  a  owl:ObjectProperty ;
        rdfs:range       swe:Quantity ;
        skos:definition  "The measured distance of the start of the mapped interval along the path of the borehole. The measured value must be less than or equal to the intervalEnd value. The \"intervalBegin\" and \"intervalEnd\" elements are added in version 3.2 as a measure to overcome problems with the delivery and queryability of 1D GML shapes via the \"interval\" element."@en .

gsmlbh:indexData  a      owl:ObjectProperty ;
        rdfs:range       gsmlbh:BoreholeDetails ;
        skos:definition  "Specifies the Borehole details"@en .

gsmlbh:referenceLocation
        a                owl:ObjectProperty ;
        rdfs:range       gsmlbh:OriginPosition ;
        skos:definition  "A Borehole OriginPosition is a feature corresponding to the start point of a borehole log.  This may, but not necessarily, correspond to the borehole collar location (eg, kelly bush)."@en .

gsmlbh:mappedIntervalBegin
        a                owl:ObjectProperty ;
        rdfs:range       swe:Quantity ;
        skos:definition  "The measured distance of the start of the mapped interval along the path of the borehole. The measured value must be less than or equal to the mappedIntervalEnd value.  The \"mappedIntervalBegin\" and \"mappedIntervalEnd\" elements are added in version 3.2 as a measure to overcome problems with the delivery and queryability of 1D GML shapes via the \"shape\" property."@en .

gsmlbh:interval  a       owl:ObjectProperty ;
        rdfs:range       gsp:Geometry ;
        skos:definition  "A shape that is a 1-D interval (eg, a \"from\" and \"to\", or \"top\" and \"base\" measurement) and uses the SRS of the containing borehole"@en .

gsmlbh:OriginPosition
        a                owl:Class ;
        rdfs:subClassOf  [ a                  owl:Restriction ;
                           owl:allValuesFrom  gsmlbh:Borehole ;
                           owl:onProperty     gsmlbh:relatedBorehole
                         ] ;
        rdfs:subClassOf  [ a                  owl:Restriction ;
                           owl:allValuesFrom  gsp:Geometry ;
                           owl:onProperty     gsmlbh:elevation
                         ] ;
        rdfs:subClassOf  [ a                  owl:Restriction ;
                           owl:allValuesFrom  gsp:Geometry ;
                           owl:onProperty     gsmlbh:location
                         ] ;
        skos:definition  "A Borehole OriginPosition is a feature corresponding to the start point of a borehole log.  This may, but not necessarily, correspond to the borehole collar location (eg, kelly bush).\r\n\r\nIf a text descripiton of the location is available, it should be placed in the gml:description for that feature.  If no GM_Point is available, an OGC nil value should be used.\r\n\r\nImplementers delivering 3-D origin locations should provide an elevation to improve interoperability. \r\n\r\nIn situations where the origin position changes over the life of the borehole (eg, due to subsidence or destruction of the original collar), the origin position should be updated to the new location."@en .

gsmlbh:DrillingDetails
        a                owl:Class ;
        rdfs:subClassOf  [ a                  owl:Restriction ;
                           owl:allValuesFrom  swe:Quantity ;
                           owl:onProperty     gsmlbh:intervalEnd
                         ] ;
        rdfs:subClassOf  [ a                  owl:Restriction ;
                           owl:allValuesFrom  swe:Quantity ;
                           owl:onProperty     gsmlbh:intervalBegin
                         ] ;
        rdfs:subClassOf  [ a                  owl:Restriction ;
                           owl:allValuesFrom  gsp:Geometry ;
                           owl:onProperty     gsmlbh:interval
                         ] ;
        rdfs:subClassOf  [ a                  owl:Restriction ;
                           owl:allValuesFrom  swe:Quantity ;
                           owl:onProperty     gsmlbh:boreholeDiameter
                         ] ;
        rdfs:subClassOf  [ a                  owl:Restriction ;
                           owl:allValuesFrom  skos:Concept ;
                           owl:onProperty     gsmlbh:drillingMethod
                         ] .

gsmlbh:relatedBorehole
        a                owl:ObjectProperty ;
        rdfs:range       gsmlbh:Borehole ;
        skos:definition  "The hole that has this collar for its start point"@en .
