@prefix rdf:   <http://www.w3.org/1999/02/22-rdf-syntax-ns#> .
@prefix owl:   <http://www.w3.org/2002/07/owl#> .
@prefix xsd:   <http://www.w3.org/2001/XMLSchema#> .
@prefix skos:  <http://www.w3.org/2004/02/skos/core#> .
@prefix gsmlv: <http://geosciml.org/ont/gsmlv#> .
@prefix rdfs:  <http://www.w3.org/2000/01/rdf-schema#> .

gsmlv:VocabRelation  a   owl:Class ;
        rdfs:subClassOf  [ a                  owl:Restriction ;
                           owl:allValuesFrom  gsmlv:GeologicVocabulary ;
                           owl:onProperty     gsmlv:VocabRelation.vocabulary
                         ] ;
        rdfs:subClassOf  [ a                  owl:Restriction ;
                           owl:allValuesFrom  skos:Concept ;
                           owl:onProperty     gsmlv:source
                         ] ;
        rdfs:subClassOf  [ a                  owl:Restriction ;
                           owl:allValuesFrom  skos:Concept ;
                           owl:onProperty     gsmlv:target
                         ] ;
        rdfs:subClassOf  [ a                  owl:Restriction ;
                           owl:allValuesFrom  rdfs:Resource ;
                           owl:onProperty     gsmlv:role
                         ] ;
        skos:definition  "Relationships between ControlledConcepts. Use to implement thesaurus type relationships like 'broader than', 'narrower than', 'related term', 'synonym' etc. role attribute specifies relationship from source to target, read 'source' 'role' 'target'. \r\n\r\nVocabRelation and some other components may be replaced by another mechanism (OWL, SKOS, RDF, etc) at some future date, according to maturity and adoption level of standard technologies"@en .

gsmlv:VocabRelation.vocabulary
        a            owl:ObjectProperty ;
        rdfs:domain  gsmlv:VocabRelation ;
        rdfs:range   gsmlv:GeologicVocabulary .

gsmlv:GeologicVocabulary
        a                owl:Class ;
        skos:definition  "A collection of terms (ControlledConcepts) and their associated definitions and relationships between the terms, usually organized in some logical fashion such as in a hierarchy (geologic time, rocks, unconsolidated deposits...).   An instance of a GeologicConcept may occur only once in a particular GeologicVocabulary.\r\n\r\nIn GeoSciML this is normally identified using a URN in the \"classifierScheme\" branch of the CGI URN scheme, with the @codesSpace attribute set to \"urn:ieft:rfc:2141\"."@en .

gsmlv:StratigraphicLexicon
        a                owl:Class ;
        rdfs:subClassOf  gsmlv:GeologicVocabulary ;
        skos:definition  "Geologic vocabulary that is a collection of ControlledConcepts that have (or could have...) GeologicFeature.GeologicUnit prototoype instances."@en .

gsmlv:target  a          owl:ObjectProperty ;
        rdfs:range       skos:Concept ;
        skos:definition  "The 'target' ControlledConcept in theVocabRelation relationship."@en .

gsmlv:role  a            owl:ObjectProperty ;
        rdfs:range       rdfs:Resource ;
        skos:definition  "Term that specifies the relationship between source and target vocabulary terms. Terms should be constructed so the source to target reading of the relationship is clear, for example SourceIsBroaderTerm, SourceIsChildOfTarget."@en .

gsmlv:source  a          owl:ObjectProperty ;
        rdfs:range       skos:Concept ;
        skos:definition  "The 'source' ControlledConcept in theVocabRelation relationship."@en .

<http://geosciml.org/ont/gsmlv>
        a                owl:Ontology ;
        owl:versionIRI   "http://geosciml.org/ont/gsmlv/3.0.0" ;
        owl:versionInfo  "3.0.0" ;
        skos:definition  "The GeoSciML Vocabulary package contains classes to support definitions and classifications. \r\n\r\nThis package is a conceptual only, and is implemented using SKOS-RDF encoded vocabularies, and URI's to link by reference to controlled concepts which define classifiers."@en .
